vale/code/arch/x64/Interop.fsti
@@ -2,7 +2,6 @@ module Interop
 module List = FStar.List.Tot.Base
 module HS = FStar.Monotonic.HyperStack
 module HH = FStar.Monotonic.HyperHeap
-module B = LowStar.Buffer
 module MB = LowStar.Monotonic.Buffer
 module M = LowStar.Modifies
 
