vale/code/arch/x64/interop/new/Vale.AsLowStar.Wrapper.fst
@@ -61,6 +61,7 @@ let rec args_b8_lemma (args:list arg) (x:arg)
       (List.memP x args ==>
         (match x with
          | (| TD_Buffer bt _, x |) -> List.memP (Buffer x true) (args_b8 args)
+         | (| TD_ImmBuffer bt _, x |) -> List.memP (imm_to_b8 x) (args_b8 args)
          | _ -> True))
   = match args with
     | [] -> ()
@@ -75,6 +76,8 @@ let arg_is_registered_root (s:ME.mem) (a:arg) =
   match a with
   | (| TD_Buffer bt _, x |) ->
     List.memP (Buffer x true) (ptrs_of_mem (as_mem s))
+  | (| TD_ImmBuffer bt _, x |) ->
+    List.memP (imm_to_b8 x) (ptrs_of_mem (as_mem s))    
   | _ -> true
 
 let core_create_lemma_readable
@@ -93,8 +96,10 @@ let core_create_lemma_readable
       = match a with
         | (| TD_Buffer bt _, x |) ->
           Vale.AsLowStar.MemoryHelpers.reveal_readable #bt x s;
-          Vale.AsLowStar.MemoryHelpers.buffer_writeable_reveal bt x          
-        | _ -> ()
+          Vale.AsLowStar.MemoryHelpers.buffer_writeable_reveal bt x
+        | (| TD_ImmBuffer bt _, x |) ->
+          Vale.AsLowStar.MemoryHelpers.reveal_imm_readable #bt x s
+        | (| TD_Base _, _ |) -> ()
     in
     let rec readable_registered_all
         (args:list arg)
@@ -125,7 +130,9 @@ let readable_live_one (m:ME.mem) (a:arg)
   = match a with
     | (| TD_Buffer bt _, x |) ->
       Vale.AsLowStar.MemoryHelpers.readable_live #bt x m
-    | _ -> ()
+    | (| TD_ImmBuffer bt _, x |) ->
+      Vale.AsLowStar.MemoryHelpers.readable_imm_live #bt x m
+    | (| TD_Base _, _ |) -> ()
 
 let rec readable_all_live (m:ME.mem) (args:list arg)
   : Lemma (VSig.readable args m ==>
@@ -169,9 +176,10 @@ let core_create_lemma_mem_correspondance
     | hd::tl -> aux tl;
       match hd with
       | (| TD_Buffer bt _, x |) ->
-        let open Vale.AsLowStar.MemoryHelpers in
-        buffer_as_seq_reveal bt x args h0 stack
-      | _ -> ()
+        Vale.AsLowStar.MemoryHelpers.buffer_as_seq_reveal bt x args h0 stack
+      | (| TD_ImmBuffer bt _, x |) ->
+        Vale.AsLowStar.MemoryHelpers.immbuffer_as_seq_reveal bt x args h0 stack      
+      | (| TD_Base _, _ |) -> ()
     in
     aux args
 
@@ -251,7 +259,8 @@ let core_create_lemma_register_args
         let (| tag, x |) = hd in
         match tag with
         | TD_Buffer bt _ -> Vale.AsLowStar.MemoryHelpers.buffer_addr_reveal bt x args' h0
-        | _ -> ()
+        | TD_ImmBuffer bt _ -> Vale.AsLowStar.MemoryHelpers.immbuffer_addr_reveal bt x args' h0
+        | TD_Base _ -> ()
       in
       aux args va_s (arg_of_sb stack::args) h0
 
@@ -334,9 +343,9 @@ let rec frame_mem_correspondence_back
    | hd::tl ->
      frame_mem_correspondence_back tl h0 h1 va_s l;
      match hd with
-     | (| TD_Buffer bt _, x |) ->
+     | (| TD_Buffer bt _, x |) | (| TD_ImmBuffer bt _, x |) ->
        BufferViewHelpers.lemma_bv_equal (LSig.view_of_base_typ bt) x h0 h1
-     | _ -> ()
+     | (| TD_Base _, _ |) -> ()
 
 let rec frame_mem_correspondence
        (args:list arg)
@@ -357,9 +366,9 @@ let rec frame_mem_correspondence
    | hd::tl ->
      frame_mem_correspondence tl h0 h1 va_s l;
      match hd with
-     | (| TD_Buffer bt _, x |) ->
+     | (| TD_Buffer bt _, x |) | (| TD_ImmBuffer bt _, x |) ->
        BufferViewHelpers.lemma_bv_equal (LSig.view_of_base_typ bt) x h0 h1
-     | _ -> ()
+     | (| TD_Base _, _ |) -> ()
 
 let rec args_fp (args:list arg)
                 (h0:mem_roots args)
@@ -368,7 +377,11 @@ let rec args_fp (args:list arg)
       (B.loc_disjoint (loc_all_args args) (B.loc_regions false (Set.singleton (HS.get_tip h1))))
   = match args with
     | [] -> ()
-    | hd::tl -> args_fp tl h0 h1
+    | hd::tl -> args_fp tl h0 h1; 
+      match hd with
+      | (| TD_Buffer _ _, _ |) | (| TD_Base _, _ |) -> ()
+      | (| TD_ImmBuffer _ _, x |) -> 
+        assert (B.loc_includes (B.loc_not_unused_in h0) (B.loc_buffer x))
 
 let eval_code_ts (c:TS.tainted_code)
                  (s0:TS.traceState)
@@ -396,6 +409,8 @@ let rec mem_correspondence_refl (args:list arg)
      match hd with
      | (| TD_Buffer bt _, x |) ->
        Vale.AsLowStar.MemoryHelpers.buffer_as_seq_reveal2 bt x va_s
+     | (| TD_ImmBuffer bt _, x |) ->
+       Vale.AsLowStar.MemoryHelpers.immbuffer_as_seq_reveal2 bt x va_s
      | _ -> ()
 
 ////////////////////////////////////////////////////////////////////////////////
