vale/code/arch/x64/interop/new/X64.MemoryAdapters.fsti
@@ -11,6 +11,7 @@ module V = X64.Vale.Decls
 module TS = X64.Taint_Semantics_s
 
 val as_vale_buffer (#t:_) (i:IB.buf_t t) : ME.buffer t
+val as_vale_immbuffer (#t:_) (i:IB.ibuf_t t) : ME.buffer t
 
 val mem_eq : squash (ME.mem == IB.mem)
 
